theories/Unification.v
@@ -1,0 +1,553 @@
+(******************************************************************************)
+(* Copyright (c) 2022 Steven Keuchel                                          *)
+(* All rights reserved.                                                       *)
+(*                                                                            *)
+(* Redistribution and use in source and binary forms, with or without         *)
+(* modification, are permitted provided that the following conditions are     *)
+(* met:                                                                       *)
+(*                                                                            *)
+(* 1. Redistributions of source code must retain the above copyright notice,  *)
+(*    this list of conditions and the following disclaimer.                   *)
+(*                                                                            *)
+(* 2. Redistributions in binary form must reproduce the above copyright       *)
+(*    notice, this list of conditions and the following disclaimer in the     *)
+(*    documentation and/or other materials provided with the distribution.    *)
+(*                                                                            *)
+(* THIS SOFTWARE IS PROVIDED BY THE COPYRIGHT HOLDERS AND CONTRIBUTORS        *)
+(* "AS IS" AND ANY EXPRESS OR IMPLIED WARRANTIES, INCLUDING, BUT NOT LIMITED  *)
+(* TO, THE IMPLIED WARRANTIES OF MERCHANTABILITY AND FITNESS FOR A PARTICULAR *)
+(* PURPOSE ARE DISCLAIMED. IN NO EVENT SHALL THE COPYRIGHT HOLDER OR          *)
+(* CONTRIBUTORS BE LIABLE FOR ANY DIRECT, INDIRECT, INCIDENTAL, SPECIAL,      *)
+(* EXEMPLARY, OR CONSEQUENTIAL DAMAGES (INCLUDING, BUT NOT LIMITED TO,        *)
+(* PROCUREMENT OF SUBSTITUTE GOODS OR SERVICES; LOSS OF USE, DATA, OR         *)
+(* PROFITS; OR BUSINESS INTERRUPTION) HOWEVER CAUSED AND ON ANY THEORY OF     *)
+(* LIABILITY, WHETHER IN CONTRACT, STRICT LIABILITY, OR TORT (INCLUDING       *)
+(* NEGLIGENCE OR OTHERWISE) ARISING IN ANY WAY OUT OF THE USE OF THIS         *)
+(* SOFTWARE, EVEN IF ADVISED OF THE POSSIBILITY OF SUCH DAMAGE.               *)
+(******************************************************************************)
+
+From Coq Require Import
+     Arith.PeanoNat
+     Classes.CRelationClasses
+     Program.Tactics.
+From Equations Require Import
+     Equations.
+From Equations.Type Require
+     Classes
+     WellFounded.
+From Equations.Prop Require
+     Classes.
+From MasterThesis Require Import
+     Context Environment Prelude.
+Import ctx.
+Import ctx.notations.
+Import SigTNotations.
+
+Set Implicit Arguments.
+
+Definition TYPE : Type := Ctx nat -> Type.
+Definition Valid (A : TYPE) : Type :=
+  forall Σ, A Σ.
+Definition Impl (A B : TYPE) : TYPE :=
+  fun Σ => A Σ -> B Σ.
+Definition Forall {I : Type} (A : I -> TYPE) : TYPE :=
+  fun w => forall i : I, A i w.
+
+Definition Unit : TYPE := fun _ => unit.
+Definition Option (A : TYPE) : TYPE := fun Σ => option (A Σ).
+Definition Prod (A B : TYPE) : TYPE := fun Σ => prod (A Σ) (B Σ).
+Definition Sum (A B : TYPE) : TYPE := fun Σ => sum (A Σ) (B Σ).
+
+Inductive Ty (Σ : Ctx nat) : Type :=
+  | t_evar (x : nat) (xIn : x ∈ Σ)
+  | t_bool
+  | t_func (T1 T2 : Ty Σ).
+Arguments t_evar {Σ x} xIn.
+Arguments t_bool {Σ}.
+Arguments t_func {Σ}.
+
+Derive NoConfusion for Ty.
+
+Module Tri.
+
+  Inductive Tri (Σ : Ctx nat) : Ctx nat -> Set :=
+  | refl      : Tri Σ Σ
+  | cons {Σ' x} (xIn : x ∈ Σ) (t : Ty (Σ - x)%ctx) (ζ : Tri (Σ - x) Σ') : Tri Σ Σ'.
+  Global Arguments refl {_}.
+  Global Arguments cons {_ _} x {_} t ζ.
+
+  Fixpoint trans [Σ0 Σ1 Σ2] (ζ : Tri Σ0 Σ1) {struct ζ} : Tri Σ1 Σ2 -> Tri Σ0 Σ2 :=
+     match ζ with
+     | refl       => fun ξ => ξ
+     | cons x t ν => fun ξ => cons x t (trans ν ξ)
+     end.
+
+  #[export] Instance preorder_tri : CRelationClasses.PreOrder Tri :=
+    {| PreOrder_Reflexive Σ := refl;
+       PreOrder_Transitive  := trans
+    |}.
+
+End Tri.
+Notation "Σ1 ⊒ Σ2" := (Tri.Tri Σ1 Σ2) (at level 80).
+
+Definition Box (A : TYPE) : TYPE :=
+  fun w0 => forall w1, w0 ⊒ w1 -> A w1.
+Definition Diamond (A : TYPE) : TYPE :=
+  fun w0 => {w1 : Ctx nat & ((w0 ⊒ w1) * A w1)}%type.
+Definition DiamondT (M : TYPE -> TYPE) : TYPE -> TYPE :=
+  fun A => M (fun w0 => {w1 : Ctx nat & ((w0 ⊒ w1) * A w1)}%type).
+
+Definition Later (A : TYPE) : TYPE :=
+  fun Γ => forall x (xIn : x ∈ Γ), A (Γ - x).
+Definition LaterTm (A : TYPE) : TYPE :=
+  fun Γ => forall x (xIn : x ∈ Γ), Ty (Γ - x) -> A (Γ - x).
+Definition Sooner (A : TYPE) : TYPE :=
+  fun Γ => sigT (fun x => sigT (fun (xIn : x ∈ Γ) => A (Γ - x))).
+Definition SoonerTm (A : TYPE) : TYPE :=
+  fun Γ => sigT (fun x => sigT (fun (xIn : x ∈ Γ) => Ty (Γ - x) * A (Γ - x)))%type.
+
+
+Notation "◅ A" := (Sooner A) (at level 9, right associativity).
+Notation "◄ A" := (SoonerTm A) (at level 9, right associativity).
+
+Notation "□ A" := (Box A) (at level 9, format "□ A", right associativity).
+Notation "◇ A" := (DiamondT id A) (at level 9, format "◇ A", right associativity).
+Notation "? A" := (Option A) (at level 9, format "? A", right associativity).
+Notation "◆ A" := (DiamondT Option A) (at level 9, format "◆ A", right associativity).
+Notation "A * B" := (Prod A B).
+
+Notation "⊢ A" := (Valid A) (at level 100).
+Notation "A -> B" := (Impl A B).
+Notation "'∀' x .. y , P " :=
+  (Forall (fun x => .. (Forall (fun y => P)) ..))
+    (at level 99, x binder, y binder, right associativity).
+Notation "▻ A" := (Later A) (at level 9, right associativity).
+Notation "► A" := (LaterTm A) (at level 9, right associativity).
+
+Section Löb.
+
+  Context (P : TYPE) (step : ⊢ ▻P -> P).
+
+  Obligation Tactic := auto using Nat.eq_le_incl, length_remove.
+  Equations(noeqns) Löb {Σ : Ctx nat} : P Σ by wf (length Σ) :=
+  Löb := step (fun _ _ => Löb).
+
+End Löb.
+Arguments Löb P step Σ : clear implicits.
+
+Definition K {A B} :
+  ⊢ □(A -> B) -> (□A -> □B) :=
+  fun w0 f a w1 ω01 =>
+    f w1 ω01 (a w1 ω01).
+Definition T {A} :
+  ⊢ □A -> A :=
+  fun w0 a => a w0 Tri.refl.
+Definition four {A} :
+  ⊢ □A -> □□A :=
+  fun w0 a w1 ω01 w2 ω12 =>
+    a w2 (Tri.trans ω01 ω12).
+Global Arguments four : simpl never.
+Definition D {A} : ⊢ □A -> ◇A :=
+  fun Σ a => existT _ Σ (Tri.refl, T a).
+
+Definition box2later {A} : ⊢ □A -> ►A.
+  intros Σ a x xIn t. apply a. econstructor.
+  apply t. constructor.
+Defined.
+
+Definition sooner2diamond {A} : ⊢ ◄A -> ◇A.
+  intros Σ a. destruct a as [σ [σIn [t a]]].
+  econstructor. split; try eassumption.
+  econstructor 2. auto. constructor 1.
+Defined.
+
+Definition sooner2diamondtm {A} : ⊢ ◄A -> ◆A.
+  intros Σ a. destruct a as [σ [σIn [t a]]].
+  constructor.
+  econstructor. split; try eassumption.
+  econstructor 2. auto. constructor 1.
+Defined.
+
+Definition η {A} : ⊢ A -> ◆A :=
+  fun Σ a => Some (existT _ Σ (Tri.refl, a)).
+Arguments η {A Σ} a.
+
+Definition η1 {A} {Σ x} {xIn : x ∈ Σ} (t : Ty (Σ - x)) (a : A (Σ - x)) : ◆A Σ :=
+  sooner2diamondtm (existT _ x (existT _ xIn (t, a))).
+
+Section Thick.
+
+  Definition thick : ⊢ Ty -> ►Ty :=
+    fun Σ =>
+      fix thick (S : Ty Σ) (x : nat) (xIn : x ∈ Σ) (T : Ty (Σ - x)) {struct S} : Ty (Σ - x) :=
+      match S with
+      | t_evar σIn   => match occurs_check_view xIn σIn with
+                        | Same _     => T
+                        | Diff _ yIn => t_evar yIn
+                        end
+      | t_bool       => t_bool
+      | t_func S1 S2 => t_func (thick S1 x xIn T) (thick S2 x xIn T)
+      end.
+
+End Thick.
+
+Arguments thick {_} s x {_} u.
+Notation "s [ x ↦ u ]" := (thick s x u)
+  (at level 8, left associativity,
+   format "s [ x ↦ u ]").
+
+Section Thin.
+
+  Fixpoint thin {Σ x} (xIn : x ∈ Σ) (T : Ty (Σ - x)) : Ty Σ :=
+    match T with
+    | t_evar yIn => t_evar (in_thin xIn yIn)
+    | t_bool => t_bool
+    | t_func T1 T2 => t_func (thin xIn T1) (thin xIn T2)
+    end.
+
+  Definition fancy_thin : ⊢ ◅Ty -> Ty :=
+    fun Σ '(x; (xIn; T)) => thin xIn T.
+
+End Thin.
+
+Lemma thin_thick {Σ y} (yIn : y ∈ Σ) (s t : Ty (Σ - y)) :
+  (thin yIn t)[y↦s] = t.
+Proof.
+  induction t; cbn; f_equal; auto.
+  now rewrite occurs_check_view_thin.
+Qed.
+
+Section OccursCheck.
+  Import option.notations.
+
+  Definition occurs_check_in : ⊢ ∀ x, In x -> ▻(Option (In x)) :=
+    fun w x xIn y yIn =>
+      match occurs_check_view yIn xIn with
+      | Same _      => None
+      | Diff _ xIn' => Some xIn'
+      end.
+
+  Definition occurs_check : ⊢ Ty -> ▻(Option Ty) :=
+    fun w =>
+      fix oc (t : Ty w) (y : nat) (yIn : y ∈ w) {struct t} :=
+      match t with
+      | t_evar xIn   => Some t_evar <*> occurs_check_in xIn yIn
+      | t_bool       => Some t_bool
+      | t_func T1 T2 => Some t_func <*> oc T1 y yIn <*> oc T2 y yIn
+      end.
+
+  Lemma occurs_check_thin {Σ x} (xIn : x ∈ Σ) (t : Ty (Σ - x)) :
+    option.wp (eq t) (occurs_check (thin xIn t) xIn).
+  Proof.
+    induction t; cbn.
+    - rewrite option.wp_map. unfold occurs_check_in.
+      rewrite occurs_check_view_thin. now constructor.
+    - now constructor.
+    - repeat rewrite ?option.wp_aplazy, ?option.wp_map.
+      repeat option.tactics.mixin. congruence.
+  Qed.
+
+  Lemma occurs_check_sound {Σ} (t : Ty Σ) {x} (xIn : x ∈ Σ) :
+    option.wlp (fun t' => t = thin xIn t') (occurs_check t xIn).
+  Proof.
+    induction t; cbn.
+    - unfold occurs_check_in.
+      now destruct occurs_check_view; constructor.
+    - now constructor.
+    - repeat rewrite ?option.wlp_aplazy, ?option.wlp_map.
+      repeat option.tactics.mixin. cbn. congruence.
+  Qed.
+
+End OccursCheck.
+
+Definition box_intro_split {A} :
+  ⊢ A -> ►□A -> □A :=
+  fun Σ0 a la Σ1 ζ =>
+    match ζ with
+    | Tri.refl => a
+    | Tri.cons x t ζ' => la x _ t _ ζ'
+    end.
+
+Definition SUBST : TYPE := Ty -> □Ty.
+Section Subst.
+
+  Context [Σ] (lsubst : ▻(Ty -> □Ty) Σ).
+
+  Definition subst_in {x} (xIn : In x Σ) : □Ty Σ :=
+    box_intro_split
+      (t_evar xIn)
+      (fun y yIn s =>
+         match occurs_check_view yIn xIn with
+         | Same _     => lsubst yIn s
+         | Diff _ xIn => lsubst yIn (t_evar xIn)
+         end).
+
+  Definition subst : Ty Σ -> □Ty Σ :=
+    fix subst (t : Ty Σ) : □Ty Σ :=
+      match t with
+      | t_evar xIn   => subst_in xIn
+      | t_bool       => fun _ _ => t_bool
+      | t_func T1 T2 => fun _ ζ => t_func (subst T1 _ ζ) (subst T2 _ ζ)
+      end.
+
+End Subst.
+
+Definition realsubst_fast : ⊢ Ty -> □Ty :=
+  Löb SUBST subst.
+
+Definition realsubst_slow : ⊢ Ty -> □Ty.
+  refine (fix subst {Σ} (t : Ty Σ) {Σ1} ζ1 {struct ζ1} := _).
+  destruct ζ1.
+  - apply t.
+  - refine (subst _ _ _ ζ1).
+    apply (thick t).
+    apply t0.
+Defined.
+
+Definition Hom (A B : TYPE) := ⊢ A -> B.
+
+Definition fmap {A B} (f : Hom A B) : Hom ◆A ◆B.
+Proof.
+  intros Σ0 [[Σ1 [ζ1 a1]]|].
+  - constructor 1. exists Σ1. split. auto. apply f. auto.
+  - constructor 2.
+Defined.
+(* Notation "f <$> a" := (fmap f a) (at level 20). *)
+
+Section Mult.
+  Import option.notations.
+
+  Definition μ {A} : Hom ◆◆A ◆A :=
+    fun Σ0 a0 =>
+      '(Σ1; (ζ1 , a1)) <- a0;;
+      '(Σ2; (ζ2 , a2)) <- a1;;
+      Some (Σ2; (Tri.trans ζ1 ζ2, a2)).
+
+  Definition ebind {A B} : Hom A ◆B -> Hom ◆A ◆B :=
+    fun f Σ0 a0 =>
+      '(Σ1; (ζ1, a1)) <- a0 ;;
+      '(Σ2; (ζ2, b2)) <- f Σ1 a1 ;;
+      Some (Σ2; (Tri.trans ζ1 ζ2, b2)).
+
+  Definition bind {A B} : ⊢ ◆A -> □(A -> ◆B) -> ◆B :=
+    fun Σ a0 f =>
+      '(Σ1; (ζ1 , a1)) <- a0 ;;
+      '(Σ2; (ζ2 , b2)) <- f Σ1 ζ1 a1 ;;
+      Some (Σ2; (Tri.trans ζ1 ζ2, b2)).
+
+End Mult.
+
+Notation "⟨ ζ ⟩ x <- ma ;; mb" :=
+  (bind ma (fun _ ζ x => mb))
+    (at level 80, x at next level,
+      ma at next level, mb at level 200,
+      right associativity).
+
+(* see Kobayashi, S. (1997). Monad as modality. *)
+Definition strength {A B} : Hom (□A * ◆B) (◆(□A * B)) :=
+  fun Σ0 '(a0,b0) => bind b0 (fun Σ1 ζ1 b1 => η (four a0 ζ1, b1)).
+
+Definition Assignment : TYPE :=
+  @Env nat (fun _ => Ty ctx.nil).
+Definition Lift (A : Type) : TYPE :=
+  fun Σ => (Assignment Σ -> A)%type.
+Definition Const (A : Type) : TYPE :=
+  fun _ => A.
+Definition PROP : TYPE :=
+  fun _ => Prop.
+
+Definition Property : TYPE :=
+  □PROP.
+
+Definition Unifies : ⊢ Ty -> Ty -> Property.
+  intros Σ s t Σ1 ζ1.
+  apply (realsubst_slow s ζ1 = realsubst_slow t ζ1).
+Defined.
+
+Notation "ζ ⊨ s ~ t" := (Unifies s t ζ) (at level 90, s at level 69).
+
+Definition wp {A} : ⊢ ◆A -> □(A -> PROP) -> PROP :=
+  fun Σ0 a0 POST => option.wp (fun '(Σ1; (ζ1 , a1)) => POST Σ1 ζ1 a1) a0.
+
+Definition wlp {A} : ⊢ ◆A -> □(A -> PROP) -> PROP :=
+  fun Σ0 a0 POST => option.wlp (fun '(Σ1; (ζ1 , a1)) => POST Σ1 ζ1 a1) a0.
+
+Lemma wp_η {A Σ} (a : A Σ) (POST : □(A -> PROP) Σ) :
+  wp (η a) POST <-> T POST a.
+Proof. unfold wp, η. now option.tactics.mixin. Qed.
+
+Lemma wp_μ {A B Σ} (a : ◆A Σ) (f : □(A -> ◆B) Σ) (POST : □(B -> PROP) Σ) :
+  wp (bind a f) POST <-> wp a (fun _ ζ1 a1 => wp (f _ ζ1 a1) (four POST ζ1)).
+Proof.
+  unfold wp, bind.
+  now repeat
+    (rewrite ?option.wp_bind;
+     repeat option.tactics.mixin;
+     intros; try destruct_conjs).
+Qed.
+
+Lemma wlp_η {A Σ} (a : A Σ) (POST : □(A -> PROP) Σ) :
+  wlp (η a) POST <-> T POST a.
+Proof. unfold wlp, η. now option.tactics.mixin. Qed.
+
+Lemma wlp_μ {A B Σ} (a : ◆A Σ) (f : □(A -> ◆B) Σ) (POST : □(B -> PROP) Σ) :
+  wlp (bind a f) POST <-> wlp a (fun _ ζ1 a1 => wlp (f _ ζ1 a1) (four POST ζ1)).
+Proof.
+  unfold wlp, bind.
+  now repeat
+    (rewrite ?option.wlp_bind;
+     repeat option.tactics.mixin;
+     intros; try destruct_conjs).
+Qed.
+
+Section VarView.
+
+  Inductive VarView {Σ} : Ty Σ -> Type :=
+  | is_var {x} (xIn : x ∈ Σ) : VarView (t_evar xIn)
+  | not_var {t} (H: forall x (xIn : x ∈ Σ), t <> t_evar xIn) : VarView t.
+
+  Definition varview {Σ} (t : Ty Σ) : VarView t :=
+    match t with
+    | t_evar xIn => is_var xIn
+    | _ => ltac:(constructor 2; discriminate)
+    end.
+
+  (*     apply noConfusion_inv in e. apply e. *)
+  (*     apply noConfusion_inv in e. apply e. *)
+  (*   Defined. *)
+  (*   Eval cbv [varview] in @varview. *)
+  (* Next Obligation *)
+  (* | tf_bool *)
+  (* | tf_func (T1 T2 : T Σ). *)
+  (* Global Arguments tf_bool {_ _}. *)
+  (* Global Arguments tf_func {_ _} T1 T2. *)
+
+  (* Definition Var : TYPE := *)
+  (*   fun Σ => {x & In x Σ}. *)
+
+  (* Definition unfold : ⊢ Ty -> Sum Var (TyF Ty) := *)
+  (*   fun Σ t => match t with *)
+  (*              | t_evar xIn   => inl (_;xIn) *)
+  (*              | t_bool       => inr (tf_bool) *)
+  (*              | t_func t1 t2 => inr (tf_func t1 t2) *)
+  (*              end. *)
+
+  (* Definition fold : ⊢ Sum Var (TyF Ty) -> Ty := *)
+  (*   fun Σ t => match t with *)
+  (*              | inl (_;xIn) => t_evar xIn *)
+  (*              | inr (tf_bool) => t_bool *)
+  (*              | inr (tf_func t1 t2) => t_func t1 t2 *)
+  (*              end. *)
+
+End VarView.
+
+Module Variant1.
+
+  Definition flex : ⊢ Ty -> ∀ x, In x -> ◆Unit :=
+    fun Σ t x xIn =>
+      match varview t with
+      | is_var yIn =>
+          match occurs_check_view xIn yIn with
+          | Same _      => η tt
+          | Diff _ yIn' => Some (sooner2diamond (_; (xIn; (t_evar yIn', tt))))
+          end
+      | not_var _ =>
+          option_map
+            (fun t' => sooner2diamond (x; (xIn; (t', tt))))
+            (occurs_check t xIn)
+      end.
+
+  Import option.notations.
+  Set Equations With UIP.
+  Lemma flex_sound {Σ y} (t : Ty Σ) (yIn : In y Σ) :
+    wlp (flex t yIn) (fun _ ζ1 _ => ζ1 ⊨ t ~ t_evar yIn).
+  Proof.
+    unfold Unifies, flex, wlp.
+    destruct (varview t).
+    - destruct (occurs_check_view yIn xIn); cbn.
+      + constructor. reflexivity.
+      + constructor; cbn.
+        now rewrite ?occurs_check_view_refl, ?occurs_check_view_thin.
+    - repeat rewrite ?option.wlp_aplazy, ?option.wlp_map.
+      generalize (occurs_check_sound t yIn). apply option.wlp_monotonic.
+      intros t' ->; cbn. rewrite occurs_check_view_refl.
+      apply thin_thick.
+  Qed.
+
+  Definition Unifier : TYPE :=
+    Ty -> Ty -> ◆Unit.
+  Definition BoxUnifier : TYPE :=
+    Ty -> Ty -> □◆Unit.
+
+  Section MguO.
+
+    Context [Σ] (lmgu : ▻BoxUnifier Σ).
+
+    Definition boxflex {x} (xIn : x ∈ Σ) (t : Ty Σ) : □◆Unit Σ :=
+      box_intro_split (flex t xIn) (fun z zIn u => lmgu _ (t_evar xIn)[z↦u] t[z↦u]).
+
+    Equations boxmgu : BoxUnifier Σ :=
+    | t_evar xIn   | t            := boxflex xIn t;
+    | s            | t_evar yIn   := boxflex yIn s;
+    | t_bool       | t_bool       := fun _ _ => η tt;
+    | t_func s1 s2 | t_func t1 t2 := fun _ ζ1 =>
+                                       ⟨ ζ2 ⟩ _ <- boxmgu s1 t1 ζ1 ;;
+                                       ⟨ ζ3 ⟩ _ <- boxmgu s2 t2 (Tri.trans ζ1 ζ2) ;;
+                                       η tt;
+    | _            | _            := fun _ _ => None.
+
+  End MguO.
+
+  Definition mgu : ⊢ Unifier :=
+    fun Σ s t => T (@Löb _ boxmgu Σ s t).
+
+  Lemma mgu_complete {Σ} (s t : Ty Σ) {Σ2} (ζ2 : Σ ⊒ Σ2) (HU : ζ2 ⊨ s ~ t) :
+    wp (mgu s t) (fun Σ1 ζ1 _ => exists ζ12 : Σ1 ⊒ Σ2, ζ2 = Tri.trans ζ1 ζ12).
+  Proof.
+  Admitted.
+
+End Variant1.
+
+Module Variant2.
+
+  Definition Unifier : TYPE :=
+    Ty -> Ty -> ◆Ty.
+  Definition BoxUnifier : TYPE :=
+    Ty -> Ty -> □◆Ty.
+
+  Definition flex : ⊢ Ty -> ∀ x, In x -> ◆Ty :=
+    fun Σ t x xIn =>
+      match t with
+      | t_evar yIn =>
+          match occurs_check_view xIn yIn with
+          | Same _      => η (t_evar xIn)
+          | Diff _ yIn' => Some (sooner2diamond (x; (xIn; (t_evar yIn', t_evar yIn'))))
+          end
+      | _ => option_map
+               (fun t' => sooner2diamond (x; (xIn; (t', t'))))
+               (occurs_check t xIn)
+      end.
+
+  Section MguO.
+
+    Context [Σ] (lmgu : ▻BoxUnifier Σ).
+
+    Definition boxflex {x} (xIn : x ∈ Σ) (t : Ty Σ) : □◆Ty Σ :=
+      box_intro_split (flex t xIn) (fun z zIn u => lmgu _ (t_evar xIn)[z↦u] t[z↦u]).
+
+    Equations boxmgu : BoxUnifier Σ :=
+    | t_evar xIn   | t            := boxflex xIn t;
+    | s            | t_evar yIn   := boxflex yIn s;
+    | t_bool       | t_bool       := fun _ _ => η t_bool;
+    | t_func s1 s2 | t_func t1 t2 := fun _ ζ1 =>
+                                       ⟨ ζ2 ⟩ r1 <- boxmgu s1 t1 ζ1 ;;
+                                       ⟨ ζ3 ⟩ r2 <- boxmgu s2 t2 (Tri.trans ζ1 ζ2) ;;
+                                       η (t_func (realsubst_slow r1 ζ3) r2);
+    | _            | _            := fun _ _ => None.
+
+  End MguO.
+
+  Definition mgu : ⊢ Unifier :=
+    fun Σ s t => T (@Löb _ boxmgu Σ s t).
+
+End Variant2.
